BFT_RGA.scala
@@ -1,0 +1,489 @@
+object BFT_RGA {
+
+def list_all[A](p : A => Boolean, x1 : List[A]) : Boolean = (p, x1) match {
+  case (p, Nil) => true
+  case (p, x :: xs) => p(x) && list_all[A](p, xs)
+}
+
+abstract sealed class set[A]
+final case class seta[A](a : List[A]) extends set[A]
+final case class coset[A](a : List[A]) extends set[A]
+
+trait equal[A] {
+  val `BFT_RGA.equal` : (A, A) => Boolean
+}
+def equal[A](a : A, b : A)(implicit A: equal[A]) : Boolean =
+  A.`BFT_RGA.equal`(a, b)
+object equal {
+  implicit def `BFT_RGA.equal_integer` : equal[BigInt] = new equal[BigInt] {
+    val `BFT_RGA.equal` = (a : BigInt, b : BigInt) => a == b
+  }
+  implicit def `BFT_RGA.equal_prod`[A : equal, B : equal] : equal[(A, B)] = new
+    equal[(A, B)] {
+    val `BFT_RGA.equal` = (a : (A, B), b : (A, B)) => equal_proda[A, B](a, b)
+  }
+  implicit def
+    `BFT_RGA.equal_operation`[A : equal, B : equal,
+                               C : equal] : equal[operation[A, B, C]]
+    = new equal[operation[A, B, C]] {
+    val `BFT_RGA.equal` = (a : operation[A, B, C], b : operation[A, B, C]) =>
+      equal_operationa[A, B, C](a, b)
+  }
+  implicit def `BFT_RGA.equal_literal` : equal[String] = new equal[String] {
+    val `BFT_RGA.equal` = (a : String, b : String) => a == b
+  }
+  implicit def `BFT_RGA.equal_fset`[A : equal] : equal[fset[A]] = new
+    equal[fset[A]] {
+    val `BFT_RGA.equal` = (a : fset[A], b : fset[A]) => equal_fseta[A](a, b)
+  }
+}
+
+def eq[A : equal](a : A, b : A) : Boolean = equal[A](a, b)
+
+def membera[A : equal](x0 : List[A], y : A) : Boolean = (x0, y) match {
+  case (Nil, y) => false
+  case (x :: xs, y) => eq[A](x, y) || membera[A](xs, y)
+}
+
+def member[A : equal](x : A, xa1 : set[A]) : Boolean = (x, xa1) match {
+  case (x, coset(xs)) => ! (membera[A](xs, x))
+  case (x, seta(xs)) => membera[A](xs, x)
+}
+
+def less_eq_set[A : equal](a : set[A], b : set[A]) : Boolean = (a, b) match {
+  case (coset(Nil), seta(Nil)) => false
+  case (a, coset(ys)) => list_all[A](((y : A) => ! (member[A](y, a))), ys)
+  case (seta(xs), b) => list_all[A](((x : A) => member[A](x, b)), xs)
+}
+
+abstract sealed class fset[A]
+final case class Abs_fset[A](a : set[A]) extends fset[A]
+
+def fset[A](x0 : fset[A]) : set[A] = x0 match {
+  case Abs_fset(x) => x
+}
+
+def less_eq_fset[A : equal](xa : fset[A], xc : fset[A]) : Boolean =
+  less_eq_set[A](fset[A](xa), fset[A](xc))
+
+def equal_fseta[A : equal](a : fset[A], b : fset[A]) : Boolean =
+  less_eq_fset[A](a, b) && less_eq_fset[A](b, a)
+
+trait ord[A] {
+  val `BFT_RGA.less_eq` : (A, A) => Boolean
+  val `BFT_RGA.less` : (A, A) => Boolean
+}
+def less_eq[A](a : A, b : A)(implicit A: ord[A]) : Boolean =
+  A.`BFT_RGA.less_eq`(a, b)
+def less[A](a : A, b : A)(implicit A: ord[A]) : Boolean = A.`BFT_RGA.less`(a, b)
+object ord {
+  implicit def
+    `BFT_RGA.ord_prod`[A : equal : ord, B : equal : ord] : ord[(A, B)] = new
+    ord[(A, B)] {
+    val `BFT_RGA.less_eq` = (a : (A, B), b : (A, B)) =>
+      less_eq_prod[A, B].apply(a).apply(b)
+    val `BFT_RGA.less` = (a : (A, B), b : (A, B)) =>
+      less_prod[A, B].apply(a).apply(b)
+  }
+  implicit def `BFT_RGA.ord_literal` : ord[String] = new ord[String] {
+    val `BFT_RGA.less_eq` = (a : String, b : String) => a <= b
+    val `BFT_RGA.less` = (a : String, b : String) => a < b
+  }
+}
+
+trait preorder[A] extends ord[A] {
+}
+object preorder {
+  implicit def
+    `BFT_RGA.preorder_prod`[A : equal : order,
+                             B : equal : order] : preorder[(A, B)]
+    = new preorder[(A, B)] {
+    val `BFT_RGA.less_eq` = (a : (A, B), b : (A, B)) =>
+      less_eq_prod[A, B].apply(a).apply(b)
+    val `BFT_RGA.less` = (a : (A, B), b : (A, B)) =>
+      less_prod[A, B].apply(a).apply(b)
+  }
+  implicit def `BFT_RGA.preorder_literal` : preorder[String] = new
+    preorder[String] {
+    val `BFT_RGA.less_eq` = (a : String, b : String) => a <= b
+    val `BFT_RGA.less` = (a : String, b : String) => a < b
+  }
+}
+
+trait order[A] extends preorder[A] {
+}
+object order {
+  implicit def
+    `BFT_RGA.order_prod`[A : equal : order, B : equal : order] : order[(A, B)] =
+    new order[(A, B)] {
+    val `BFT_RGA.less_eq` = (a : (A, B), b : (A, B)) =>
+      less_eq_prod[A, B].apply(a).apply(b)
+    val `BFT_RGA.less` = (a : (A, B), b : (A, B)) =>
+      less_prod[A, B].apply(a).apply(b)
+  }
+  implicit def `BFT_RGA.order_literal` : order[String] = new order[String] {
+    val `BFT_RGA.less_eq` = (a : String, b : String) => a <= b
+    val `BFT_RGA.less` = (a : String, b : String) => a < b
+  }
+}
+
+trait linorder[A] extends order[A] {
+}
+object linorder {
+  implicit def
+    `BFT_RGA.linorder_prod`[A : equal : linorder,
+                             B : equal : linorder] : linorder[(A, B)]
+    = new linorder[(A, B)] {
+    val `BFT_RGA.less_eq` = (a : (A, B), b : (A, B)) =>
+      less_eq_prod[A, B].apply(a).apply(b)
+    val `BFT_RGA.less` = (a : (A, B), b : (A, B)) =>
+      less_prod[A, B].apply(a).apply(b)
+  }
+  implicit def `BFT_RGA.linorder_literal` : linorder[String] = new
+    linorder[String] {
+    val `BFT_RGA.less_eq` = (a : String, b : String) => a <= b
+    val `BFT_RGA.less` = (a : String, b : String) => a < b
+  }
+}
+
+def equal_proda[A : equal, B : equal](x0 : (A, B), x1 : (A, B)) : Boolean =
+  (x0, x1) match {
+  case ((x1, x2), (y1, y2)) => eq[A](x1, y1) && eq[B](x2, y2)
+}
+
+def equal_option[A : equal](x0 : Option[A], x1 : Option[A]) : Boolean = (x0, x1)
+  match {
+  case (None, Some(x2)) => false
+  case (Some(x2), None) => false
+  case (Some(x2), Some(y2)) => eq[A](x2, y2)
+  case (None, None) => true
+}
+
+abstract sealed class operation[A, B, C]
+final case class Insert[C, A, B](a : C, b : A, c : Option[(A, B)]) extends
+  operation[A, B, C]
+final case class Delete[A, B, C](a : (A, B)) extends operation[A, B, C]
+
+def equal_operationa[A : equal, B : equal,
+                      C : equal](x0 : operation[A, B, C],
+                                  x1 : operation[A, B, C]) : Boolean
+  =
+  (x0, x1) match {
+  case (Insert(x11, x12, x13), Delete(x2)) => false
+  case (Delete(x2), Insert(x11, x12, x13)) => false
+  case (Delete(x2), Delete(y2)) => equal_proda[A, B](x2, y2)
+  case (Insert(x11, x12, x13), Insert(y11, y12, y13)) =>
+    eq[C](x11, y11) && (eq[A](x12, y12) && equal_option[(A, B)](x13, y13))
+}
+
+def rec_prod[A, B, C](f1 : A => B => C, x1 : (A, B)) : C = (f1, x1) match {
+  case (f1, (a, b)) => (f1(a))(b)
+}
+
+def less_eq_prod[A : equal : ord,
+                  B : equal : ord] : ((A, B)) => ((A, B)) => Boolean
+  =
+  ((x : (A, B)) => (y : (A, B)) =>
+    (rec_prod[A, B,
+               ((A, B)) =>
+                 Boolean](((x_0 : A) => (x_1 : B) => (a : (A, B)) =>
+                            {
+                              val (y_0, y_1) = a : ((A, B));
+                              less[A](x_0, y_0) ||
+                                eq[A](x_0, y_0) && less[B](x_1, y_1)
+                            }),
+                           x)).apply(y) ||
+      equal_proda[A, B](x, y))
+
+def less_prod[A : equal : ord, B : ord] : ((A, B)) => ((A, B)) => Boolean =
+  ((a : (A, B)) =>
+    rec_prod[A, B,
+              ((A, B)) =>
+                Boolean](((x_0 : A) => (x_1 : B) => (aa : (A, B)) =>
+                           {
+                             val (y_0, y_1) = aa : ((A, B));
+                             less[A](x_0, y_0) ||
+                               eq[A](x_0, y_0) && less[B](x_1, y_1)
+                           }),
+                          a))
+
+def list_ex[A](p : A => Boolean, x1 : List[A]) : Boolean = (p, x1) match {
+  case (p, Nil) => false
+  case (p, x :: xs) => p(x) || list_ex[A](p, xs)
+}
+
+def Bex[A](x0 : set[A], p : A => Boolean) : Boolean = (x0, p) match {
+  case (seta(xs), p) => list_ex[A](p, xs)
+}
+
+def Ball[A](x0 : set[A], p : A => Boolean) : Boolean = (x0, p) match {
+  case (seta(xs), p) => list_all[A](p, xs)
+}
+
+def fold[A, B](f : A => B => B, x1 : List[A], s : B) : B = (f, x1, s) match {
+  case (f, x :: xs, s) => fold[A, B](f, xs, (f(x))(s))
+  case (f, Nil, s) => s
+}
+
+def removeAll[A : equal](x : A, xa1 : List[A]) : List[A] = (x, xa1) match {
+  case (x, Nil) => Nil
+  case (x, y :: xs) =>
+    (if (eq[A](x, y)) removeAll[A](x, xs) else y :: removeAll[A](x, xs))
+}
+
+def inserta[A : equal](x : A, xs : List[A]) : List[A] =
+  (if (membera[A](xs, x)) xs else x :: xs)
+
+def insert[A : equal](x : A, xa1 : set[A]) : set[A] = (x, xa1) match {
+  case (x, coset(xs)) => coset[A](removeAll[A](x, xs))
+  case (x, seta(xs)) => seta[A](inserta[A](x, xs))
+}
+
+def filter[A](p : A => Boolean, x1 : List[A]) : List[A] = (p, x1) match {
+  case (p, Nil) => Nil
+  case (p, x :: xs) => (if (p(x)) x :: filter[A](p, xs) else filter[A](p, xs))
+}
+
+def bind[A, B](x0 : Option[A], f : A => Option[B]) : Option[B] = (x0, f) match {
+  case (None, f) => None
+  case (Some(x), f) => f(x)
+}
+
+def finsert[A : equal](xb : A, xc : fset[A]) : fset[A] =
+  Abs_fset[A](insert[A](xb, fset[A](xc)))
+
+def ref_id[A, B, C](x0 : operation[A, B, C]) : Option[A] = x0 match {
+  case Insert(v, i, ei) => Some[A](i)
+  case Delete(ei) => None
+}
+
+def delete[A : equal : linorder,
+            B](x0 : List[(A, (B, Boolean))],
+                i : A) : Option[List[(A, (B, Boolean))]]
+  =
+  (x0, i) match {
+  case (Nil, i) => None
+  case ((ia, (v, flag)) :: xs, i) =>
+    (if (eq[A](ia, i)) Some[List[(A, (B, Boolean))]]((ia, (v, true)) :: xs)
+      else bind[List[(A, (B, Boolean))],
+                 List[(A, (B, Boolean))]](delete[A, B](xs, i),
+   ((t : List[(A, (B, Boolean))]) =>
+     Some[List[(A, (B, Boolean))]]((ia, (v, flag)) :: t))))
+}
+
+def fst[A, B](x0 : (A, B)) : A = x0 match {
+  case (x1, x2) => x1
+}
+
+def insert_body[A : linorder,
+                 B](x0 : List[(A, (B, Boolean))],
+                     e : (A, (B, Boolean))) : List[(A, (B, Boolean))]
+  =
+  (x0, e) match {
+  case (Nil, e) => List(e)
+  case (x :: xs, e) =>
+    (if (less[A](fst[A, (B, Boolean)](x), fst[A, (B, Boolean)](e))) e :: x :: xs
+      else x :: insert_body[A, B](xs, e))
+}
+
+def insertb[A : equal : linorder,
+             B](xs : List[(A, (B, Boolean))], e : (A, (B, Boolean)),
+                 x2 : Option[A]) : Option[List[(A, (B, Boolean))]]
+  =
+  (xs, e, x2) match {
+  case (xs, e, None) => Some[List[(A, (B, Boolean))]](insert_body[A, B](xs, e))
+  case (Nil, e, Some(i)) => None
+  case (x :: xs, e, Some(i)) =>
+    (if (eq[A](fst[A, (B, Boolean)](x), i))
+      Some[List[(A, (B, Boolean))]](x :: insert_body[A, B](xs, e))
+      else bind[List[(A, (B, Boolean))],
+                 List[(A, (B, Boolean))]](insertb[A, B](xs, e, Some[A](i)),
+   ((t : List[(A, (B, Boolean))]) => Some[List[(A, (B, Boolean))]](x :: t))))
+}
+
+def interpret_op[A : equal : linorder, B : equal : linorder,
+                  C](h : ((fset[A], operation[B, A, C])) => A,
+                      x1 : (fset[A], operation[B, A, C]),
+                      xs : List[((B, A),
+                                  (C, Boolean))]) : Option[List[((B, A),
+                          (C, Boolean))]]
+  =
+  (h, x1, xs) match {
+  case (h, (hs, Insert(v, i, ei)), xs) =>
+    {
+      val ha = h((hs, Insert[C, B, A](v, i, ei))) : A;
+      insertb[(B, A), C](xs, ((i, ha), (v, false)), ei)
+    }
+  case (h, (hs, Delete(ei)), xs) => delete[(B, A), C](xs, ei)
+}
+
+def snd[A, B](x0 : (A, B)) : B = x0 match {
+  case (x1, x2) => x2
+}
+
+def is_rga_sem_valid[A : equal, B : equal,
+                      C](c : ((fset[A], operation[B, A, C])) =>
+                               ((fset[A], operation[B, A, C])) => Boolean,
+                          h : ((fset[A], operation[B, A, C])) => A,
+                          g : set[(fset[A], operation[B, A, C])],
+                          x3 : (fset[A], operation[B, A, C])) : Boolean
+  =
+  (c, h, g, x3) match {
+  case (c, h, g, (hs, Insert(v, i, ei))) =>
+    (ei match {
+       case None => true
+       case Some(ii) =>
+         Bex[(fset[A],
+               operation[B, A,
+                          C])](g, ((e : (fset[A], operation[B, A, C])) =>
+                                    (c(e))((hs, Insert[C, B, A](v, i, ei))) &&
+                                      (eq[A](h(e), snd[B, A](ii)) &&
+equal_option[B](ref_id[B, A, C](snd[fset[A], operation[B, A, C]](e)),
+                 Some[B](fst[B, A](ii)))))) &&
+           ! (eq[A](h((hs, Insert[C, B, A](v, i, ei))), snd[B, A](ii)))
+     })
+  case (c, h, g, (hs, Delete(ei))) =>
+    Bex[(fset[A],
+          operation[B, A,
+                     C])](g, ((e : (fset[A], operation[B, A, C])) =>
+                               (c(e))((hs, Delete[B, A, C](ei))) &&
+                                 (eq[A](h(e), snd[B, A](ei)) &&
+                                   equal_option[B](ref_id[B, A,
+                   C](snd[fset[A], operation[B, A, C]](e)),
+            Some[B](fst[B, A](ei))))))
+}
+
+def bot_set[A] : set[A] = seta[A](Nil)
+
+def sup_set[A : equal](x0 : set[A], a : set[A]) : set[A] = (x0, a) match {
+  case (coset(xs), a) =>
+    coset[A](filter[A](((x : A) => ! (member[A](x, a))), xs))
+  case (seta(xs), a) =>
+    fold[A, set[A]](((aa : A) => (b : set[A]) => insert[A](aa, b)), xs, a)
+}
+
+def is_valid[A, B](semF : (fset[(fset[A], B)]) => ((fset[A], B)) => Boolean,
+                    strF : (fset[(fset[A], B)]) => ((fset[A], B)) => Boolean,
+                    g : fset[(fset[A], B)], x : (fset[A], B)) : Boolean
+  =
+  (semF(g))(x) && (strF(g))(x)
+
+def is_rga_sem_valid_integer : (((fset[String],
+                                  operation[String, String, BigInt])) =>
+                                 ((fset[String],
+                                   operation[String, String, BigInt])) =>
+                                   Boolean) =>
+                                 (((fset[String],
+                                    operation[String, String, BigInt])) =>
+                                   String) =>
+                                   (set[(fset[String],
+  operation[String, String, BigInt])]) =>
+                                     ((fset[String],
+                                       operation[String, String, BigInt])) =>
+                                       Boolean
+  =
+  ((a : ((fset[String], operation[String, String, BigInt])) =>
+          ((fset[String], operation[String, String, BigInt])) => Boolean)
+     =>
+    (b : ((fset[String], operation[String, String, BigInt])) => String) =>
+    (c : set[(fset[String], operation[String, String, BigInt])]) =>
+    (d : (fset[String], operation[String, String, BigInt])) =>
+    is_rga_sem_valid[String, String, BigInt](a, b, c, d))
+
+def sup_fset[A : equal](xb : fset[A], xc : fset[A]) : fset[A] =
+  Abs_fset[A](sup_set[A](fset[A](xb), fset[A](xc)))
+
+def bot_fset[A] : fset[A] = Abs_fset[A](bot_set[A])
+
+def check_and_apply[A : equal,
+                     B : equal](semF : (fset[(fset[A], B)]) =>
+ ((fset[A], B)) => Boolean,
+                                 strF : (fset[(fset[A], B)]) =>
+  ((fset[A], B)) => Boolean,
+                                 x2 : (List[(fset[A], B)], fset[(fset[A], B)]),
+                                 n : (fset[A],
+                                       B)) : (List[(fset[A], B)],
+       fset[(fset[A], B)])
+  =
+  (semF, strF, x2, n) match {
+  case (semF, strF, (ah, g), n) =>
+    (if (is_valid[A, B](semF, strF, g, n))
+      (ah ++ List(n),
+        sup_fset[(fset[A],
+                   B)](g, finsert[(fset[A], B)](n, bot_fset[(fset[A], B)])))
+      else (ah, g))
+}
+
+def is_struct_valid[A : equal,
+                     B : equal](h : ((fset[A], B)) => A, g : fset[(fset[A], B)],
+                                 x2 : (fset[A], B)) : Boolean
+  =
+  (h, g, x2) match {
+  case (h, g, (hashes, vala)) =>
+    Ball[A](fset[A](hashes),
+             ((ha : A) =>
+               Bex[(fset[A],
+                     B)](fset[(fset[A], B)](g),
+                          ((n : (fset[A], B)) => eq[A](h(n), ha))))) &&
+      (! (member[(fset[A], B)]((hashes, vala), fset[(fset[A], B)](g))) &&
+        ! (member[A](h((hashes, vala)), fset[A](hashes))))
+}
+
+def rga_is_struct_valid : (((fset[String],
+                             operation[String, String, BigInt])) =>
+                            String) =>
+                            (fset[(fset[String],
+                                    operation[String, String, BigInt])]) =>
+                              ((fset[String],
+                                operation[String, String, BigInt])) =>
+                                Boolean
+  =
+  ((a : ((fset[String], operation[String, String, BigInt])) => String) =>
+    (b : fset[(fset[String], operation[String, String, BigInt])]) =>
+    (c : (fset[String], operation[String, String, BigInt])) =>
+    is_struct_valid[String, operation[String, String, BigInt]](a, b, c))
+
+def rga_check_and_apply(c : (fset[(fset[String],
+                                    operation[String, String, BigInt])]) =>
+                              ((fset[String],
+                                operation[String, String, BigInt])) =>
+                                ((fset[String],
+                                  operation[String, String, BigInt])) =>
+                                  Boolean,
+                         h : ((fset[String],
+                               operation[String, String, BigInt])) =>
+                               String) : ((List[(fset[String],
+          operation[String, String, BigInt])],
+   fset[(fset[String], operation[String, String, BigInt])])) =>
+   ((fset[String], operation[String, String, BigInt])) =>
+     (List[(fset[String], operation[String, String, BigInt])],
+       fset[(fset[String], operation[String, String, BigInt])])
+  =
+  ((a : (List[(fset[String], operation[String, String, BigInt])],
+          fset[(fset[String], operation[String, String, BigInt])]))
+     =>
+    (b : (fset[String], operation[String, String, BigInt])) =>
+    check_and_apply[String,
+                     operation[String, String,
+                                BigInt]](((g : fset[(fset[String],
+              operation[String, String, BigInt])])
+    =>
+   is_rga_sem_valid_integer.apply(c(g)).apply(h).apply(fset[(fset[String],
+                      operation[String, String, BigInt])](g))),
+  rga_is_struct_valid.apply(h), a, b))
+
+def interpret_op_integer : (((fset[String],
+                              operation[String, String, BigInt])) =>
+                             String) =>
+                             ((fset[String],
+                               operation[String, String, BigInt])) =>
+                               (List[((String, String), (BigInt, Boolean))]) =>
+                                 Option[List[((String, String),
+       (BigInt, Boolean))]]
+  =
+  ((a : ((fset[String], operation[String, String, BigInt])) => String) =>
+    (b : (fset[String], operation[String, String, BigInt])) =>
+    (c : List[((String, String), (BigInt, Boolean))]) =>
+    interpret_op[String, String, BigInt](a, b, c))
+
+} /* object BFT_RGA */
